symbolic evaluation seems to work for simple cases.

MirrorCharge!/src/Imp/SymEval.v
@@ -14,6 +14,7 @@ Require Import MirrorCore.Lambda.ExprLift.
 Require Import MirrorCore.Lambda.ExprSubst.
 Require Import MirrorCore.Lambda.ExprUnify_simul.
 Require Import MirrorCharge.Imp.Imp.
+Require Import MirrorCharge.ILogicFunc.
 
 Set Implicit Arguments.
 Set Strict Implicit.
@@ -27,22 +28,6 @@ Inductive typ :=
 | tyVariable
 | tyExpr
 | tyNat.
-
-Fixpoint typD (ls : list Type) (t : typ) : Type :=
-  match t with
-    | tyArr a b => typD ls a -> typD ls b
-    | tyLocals => locals
-    | tyCmd => icmd
-    | tyHProp => HProp
-    | tyProp => Prop
-    | tyVariable => var
-    | tyExpr => iexpr
-    | tyNat => nat
-  end.
-
-Inductive tyAcc_typ : typ -> typ -> Prop :=
-| tyAcc_tyArrL : forall a b, tyAcc_typ a (tyArr a b)
-| tyAcc_tyArrR : forall a b, tyAcc_typ a (tyArr b a).
 
 Fixpoint type_cast_typ (a b : typ) : option (a = b) :=
   match a as a , b as b return option (a = b) with
@@ -61,8 +46,34 @@ Fixpoint type_cast_typ (a b : typ) : option (a = b) :=
                 end)
         | _ , _ => None
       end
+    | tyExpr , tyExpr => Some eq_refl
+    | tyNat , tyNat => Some eq_refl
+    | tyVariable , tyVariable => Some eq_refl
     | _ , _ => None
   end.
+
+Instance RelDec_eq_typ : RelDec (@eq typ) :=
+{ rel_dec := fun a b => match type_cast_typ a b with
+                          | None => false
+                          | Some _ => true
+                        end }.
+
+Fixpoint typD (ls : list Type) (t : typ) : Type :=
+  match t with
+    | tyArr a b => typD ls a -> typD ls b
+    | tyLocals => locals
+    | tyCmd => icmd
+    | tyHProp => HProp
+    | tyProp => Prop
+    | tyVariable => var
+    | tyExpr => iexpr
+    | tyNat => nat
+  end.
+
+Inductive tyAcc_typ : typ -> typ -> Prop :=
+| tyAcc_tyArrL : forall a b, tyAcc_typ a (tyArr a b)
+| tyAcc_tyArrR : forall a b, tyAcc_typ a (tyArr b a).
+
 
 Instance RType_typ : RType typ :=
 { typD := typD
@@ -80,23 +91,45 @@ Instance Typ2_Fun : Typ2 _ Fun :=
                   end
 }.
 
+Instance Typ0_Prop : Typ0 _ Prop :=
+{ typ0 := tyProp
+; typ0_cast := fun _ => eq_refl
+; typ0_match := fun T ts t tr =>
+                  match t as t return T (typD ts t) -> T (typD ts t) with
+                    | tyProp => fun _ => tr
+                    | _ => fun fa => fa
+                  end
+}.
+
+
 Inductive imp_func :=
 | pVar (_ : var)
-| pNat (_ : nat).
+| pNat (_ : nat)
+| pLocals_get | pLocals_upd
+| pEq (_ : typ)
+| pEval_expri.
 
 (** TODO: This also needs to include logic stuff! **)
-Definition func := (SymEnv.func + imp_func)%type.
+Definition func := (SymEnv.func + imp_func + ilfunc typ)%type.
 
 Definition typeof_sym_imp (f : imp_func) : option typ :=
   Some match f with
          | pVar _ => tyVariable
          | pNat _ => tyNat
+         | pLocals_get => tyArr tyVariable (tyArr tyLocals tyNat)
+         | pLocals_upd => tyArr tyVariable (tyArr tyNat (tyArr tyLocals tyLocals))
+         | pEq t => tyArr t (tyArr t tyProp)
+         | pEval_expri => tyArr tyExpr (tyArr tyLocals tyNat)
        end.
 
 Definition imp_func_eq (a b : imp_func) : option bool :=
   match a , b with
     | pVar a , pVar b => Some (a ?[ eq ] b)
     | pNat a , pNat b => Some (a ?[ eq ] b)
+    | pLocals_get , pLocals_get => Some true
+    | pLocals_upd , pLocals_upd => Some true
+    | pEq a , pEq b => Some (a ?[ eq ] b)
+    | pEval_expri , pEval_expri => Some true
     | _ , _ => Some false
   end.
 
@@ -111,6 +144,10 @@ Instance RSym_imp_func : SymI.RSym imp_func :=
             with
               | pVar v => v
               | pNat n => n
+              | pLocals_get => locals_get
+              | pLocals_upd => locals_upd
+              | pEq t => @eq _
+              | pEval_expri => eval_iexpr
             end
 ; sym_eqb := imp_func_eq
 }.
@@ -139,15 +176,51 @@ Section tactic.
                  (fun _ => Assign) ::
        nil).
 
-  Definition RS : SymI.RSym func := SymSum.RSym_sum (SymEnv.RSym_func fs) _.
-  Definition EP : EProver2.EProver (typ := typ) (expr typ func) :=
-    EProver2.from_Prover (DefaultProver (expr typ func)).
+  Definition lops : logic_ops _ :=
+    fun t =>
+      match t
+            return option (forall ts, ILogic.ILogicOps (TypesI.typD ts t))
+      with
+        | tyProp => Some _
+        | tyHProp => Some _
+        | tyArr tyLocals tyHProp => Some (fun _ => ILogicOps_lprop)
+        | _ => None
+      end.
 
-  Definition fTriple : expr typ func := Inj (inl 1%positive).
-  Definition fSeq : expr typ func := Inj (inl 2%positive).
-  Definition fAssign : expr typ func := Inj (inl 3%positive).
-  Definition fVar (v : var) : expr typ func := Inj (inr (pVar v)).
-  Definition fConst (c : nat) : expr typ func := Inj (inr (pNat c)).
+  Definition eops : embed_ops _.
+  red. refine
+    (fun t u =>
+      match t as t , u as u
+            return option
+                     (forall ts : list Type,
+                        ILEmbed.EmbedOp (TypesI.typD ts t) (TypesI.typD ts u))
+      with
+        | tyProp , tyHProp =>
+          Some (fun _ => EmbedOp_Prop_HProp)
+        | tyHProp , tyArr tyLocals tyHProp =>
+          Some (fun ts => EmbedOp_HProp_lprop)
+        | tyProp , tyArr tyLocals tyHProp =>
+          Some (fun _ => @ILInsts.EmbedILFunDropOp _ _ EmbedOp_Prop_HProp _)
+        | _ , _ => None
+      end).
+  Defined.
+
+  Local Instance RSym_ilfunc : SymI.RSym (ilfunc typ) :=
+    @ILogicFunc.RSym_ilfunc typ _ _ lops eops _ _.
+
+  Definition RS : SymI.RSym func :=
+    SymSum.RSym_sum (SymSum.RSym_sum (SymEnv.RSym_func fs) _) _.
+  Local Existing Instance RS.
+
+  Definition fTriple : expr typ func := Inj (inl (inl 1%positive)).
+  Definition fSeq : expr typ func := Inj (inl (inl 2%positive)).
+  Definition fAssign : expr typ func := Inj (inl (inl 3%positive)).
+  Definition fVar (v : var) : expr typ func := Inj (inl (inr (pVar v))).
+  Definition fConst (c : nat) : expr typ func := Inj (inl (inr (pNat c))).
+  Definition flocals_get : expr typ func := Inj (inl (inr pLocals_get)).
+  Definition flocals_upd : expr typ func := Inj (inl (inr pLocals_upd)).
+  Definition feval_iexpr : expr typ func := Inj (inl (inr pEval_expri)).
+  Definition fEq (t : typ) : expr typ func := Inj (inl (inr (pEq t))).
 
   Definition mkTriple (P c Q : expr typ func) : expr typ func :=
     App (App (App fTriple P) c) Q.
@@ -157,14 +230,11 @@ Section tactic.
     App (App fAssign a) b.
 
   (** NOTE: Manual lemma reification for the time being **)
-  (** NOTE: This is a very difficult lemma to solve because it has multiple,
-   ** non-trivial, premises
-   **)
   Definition seq_lemma : lemma typ (expr typ func) (expr typ func) :=
   {| vars := tyLProp :: tyLProp :: tyLProp :: tyCmd :: tyCmd :: nil
-   ; premises := mkTriple (Var 4) (Var 1) (Var 3) ::
-                mkTriple (Var 3) (Var 0) (Var 2) :: nil
-   ; concl := mkTriple (Var 4) (mkSeq (Var 1) (Var 0)) (Var 2)
+   ; premises := mkTriple (Var 0) (Var 3) (Var 1) ::
+                 mkTriple (Var 1) (Var 4) (Var 2) :: nil
+   ; concl := mkTriple (Var 0) (mkSeq (Var 3) (Var 4)) (Var 2)
    |}.
 
   Definition seq_assoc_lemma : lemma typ (expr typ func) (expr typ func) :=
@@ -179,12 +249,23 @@ Section tactic.
     @eapply_other typ (expr typ func) subst tyProp vars_to_uvars
                   (fun tus tvs n e1 e2 t s =>
                      @exprUnify subst typ func _ _ RS SS SU 3 nil
-                                tus tvs n s e1 e2 t) SU.
+                                tus tvs n s e1 e2 t)
+                  (@instantiate typ func) SS SU.
 
   Definition seq_case : stac typ (expr typ func) subst :=
     FIRST (   eapply_other seq_assoc_lemma (@IDTAC _ _ _)
            :: eapply_other seq_lemma (@IDTAC _ _ _)
            :: nil).
+
+  Definition lex (l t : typ) (e : expr typ func) : expr typ func :=
+    App (Inj (inr (ilf_exists t l))) (Abs t e).
+
+  Definition land (l : typ) (e e' : expr typ func) : expr typ func :=
+    App (App (Inj (inr (ilf_and l))) e) e'.
+  Definition lor (l : typ) (e e' : expr typ func) : expr typ func :=
+    App (App (Inj (inr (ilf_or l))) e) e'.
+  Definition lembed (t f : typ) (e : expr typ func) : expr typ func :=
+    App (Inj (inr (ilf_embed f t))) e.
 
   (** Assignment **)
   Definition assign_lemma : lemma typ (expr typ func) (expr typ func) :=
@@ -193,22 +274,43 @@ Section tactic.
    ; concl :=
        mkTriple (Var 0)
                 (mkAssign (Var 1) (Var 2))
-                (Var 0)
+                (Abs tyLocals
+                     (lex tyHProp tyNat
+                          (land tyHProp
+                                (lembed tyHProp tyProp
+                                        (App (App (fEq tyNat)
+                                                  (App (App flocals_get (Var 3)) (Var 1)))
+                                             (App (App feval_iexpr (Var 4)) (Var 1))))
+                                (App (Var 2) (App (App (App flocals_upd (Var 3)) (Var 0)) (Var 1))))))
    |}.
+
+  Let Expr_expr : ExprI.Expr _ (expr typ func) := Expr_expr _ _.
+  Local Existing Instance Expr_expr.
+
+  Definition test_lemma :=
+    @lemmaD typ RType_typ (expr typ func) Expr_expr (expr typ func)
+            (fun tus tvs e => exprD' nil tus tvs tyProp e)
+            tyProp
+            (fun x => x) nil nil.
+
+(*
+  Eval compute
+    in test_lemma seq_lemma.
+*)
 
   Definition assign_case : stac typ (expr typ func) subst :=
     FIRST (   eapply_other assign_lemma (@IDTAC _ _ _)
            :: nil).
 
   Definition all_cases : stac typ (expr typ func) subst :=
-    REC 3 (fun rec =>
+    REC 2 (fun rec =>
              let rec := rec in
-             REPEAT 5
+             REPEAT 2
                     (FIRST (   eapply_other seq_assoc_lemma rec
                             :: eapply_other seq_lemma rec
                             :: eapply_other assign_lemma rec
                             :: nil)))
-        (@IDTAC _ _ _).
+        (@FAIL _ _ _).
 
   Definition test :=
     let vars := tyLProp :: tyCmd :: tyCmd :: tyCmd :: tyLProp :: nil in
@@ -220,17 +322,18 @@ Section tactic.
     @seq_case goal (SubstI3.empty (expr :=expr typ func))
               nil vars.
 
-  Time Eval vm_compute in test.
+  Definition XXX := eapply_other.
 
   Definition test' :=
+    let uvars := tyLProp :: nil in
     let vars := tyLProp :: tyVariable :: tyCmd :: tyCmd :: tyLProp :: tyExpr :: nil in
     let goal :=
         mkTriple (Var 0)
                  (mkSeq (mkAssign (Var 1) (Var 5)) (Var 2))
-                 (Var 0)
+                 (UVar 0)
     in
     @all_cases goal (SubstI3.empty (expr :=expr typ func))
-               nil vars.
+               uvars vars.
 
   Time Eval vm_compute in test'.
 
